Quiz/Quiz1209.v
@@ -1,0 +1,93 @@
+Require Import Coq.Logic.Classical_Prop.
+Require Import Coq.Strings.String.
+Require Import Coq.ZArith.ZArith.
+Require Import Coq.micromega.Psatz.
+Require Import Coq.Classes.Morphisms.
+Require Import Coq.Sorting.Permutation.
+Require Import Coq.Lists.List. Import ListNotations.
+Require Import SetsClass.SetsClass. Import SetsNotation.
+Require Import PL.Syntax.
+Require Import PL.DenotationsOfExpr.
+Require Import PL.DenotationsAsRels.
+Require Import PL.Monad.
+Require Import PL.Kleene.
+Require Import PL.FixedPoint.
+Require Import PL.MonadHoare.
+Local Open Scope Z.
+Local Open Scope list.
+
+Import Monad
+       MonadNotation
+       SetMonadExamples0
+       SetMonadExamples2
+       SetMonadExamples3
+       SetMonadHoare
+       KleeneFix Sets_CPO.
+Local Open Scope monad.
+
+(************)
+(** 习题：  *)
+(************)
+
+Definition insertion_body (x: Z):
+  list Z * list Z -> SetMonad.M (ContinueOrBreak (list Z * list Z) (list Z)) :=
+  fun '(l1, l2) =>
+    match l2 with
+    | nil => break (l1 ++ [x])
+    | cons y l2' =>
+        choice
+          (assume (x <= y);; break (l1 ++ [x] ++ l2))
+          (assume (y <= x);; continue (l1 ++ [y], l2'))
+    end.
+
+Definition insertion (x: Z) (l: list Z): SetMonad.M (list Z) :=
+  repeat_break (insertion_body x) (nil, l).
+
+Theorem insertion_perm:
+  forall x l,
+    Hoare
+      (insertion x l)
+      (fun l0 => Permutation (l ++ [x]) l0).
+Admitted. (* 请删除这一行_[Admitted]_并填入你的证明，以_[Qed]_结束。 *)
+
+Theorem insertion_incr:
+  forall x l,
+    incr l ->
+    Hoare
+      (insertion x l)
+      (fun l0 => incr l0).
+Admitted. (* 请删除这一行_[Admitted]_并填入你的证明，以_[Qed]_结束。 *)
+
+(************)
+(** 习题：  *)
+(************)
+
+Definition ins_sort (l: list Z) :=
+  list_iter insertion l nil.
+
+Theorem ins_sort_perm:
+  forall L,
+    Hoare
+      (ins_sort L)
+      (fun l => Permutation L l).
+Admitted. (* 请删除这一行_[Admitted]_并填入你的证明，以_[Qed]_结束。 *)
+
+Theorem ins_sort_incr:
+  forall L,
+    Hoare
+      (ins_sort L)
+      (fun l => incr l).
+Admitted. (* 请删除这一行_[Admitted]_并填入你的证明，以_[Qed]_结束。 *)
+
+Theorem functional_correctness_ins_sort:
+  forall L,
+    Hoare
+      (ins_sort L)
+      (fun l => Permutation L l /\ incr l).
+Proof.
+  intros.
+  apply Hoare_conjunct.
+  + apply ins_sort_perm.
+  + apply ins_sort_incr.
+Qed.
+
